

Set of equations

$$\alpha_L = -L(L+1), \quad \beta_L = -1$$

$$R_L = \left(\frac{P_L}{r} - \frac{P_L}{r} \tau_L \right) = \frac{1}{r} (P_L - \beta_L \tau_L) \quad (0)$$

$$\frac{\partial^2}{\partial r^2} U_L + P_L \left[\frac{1}{r^2} \frac{\partial}{\partial r} (r^2 U_L) + \frac{\alpha_L}{r} V_L \right] + V_L \frac{\partial R_L}{\partial r} + \frac{1}{r^2} \frac{\partial}{\partial r} (r^2 V_L) R_L = 0 \quad (1)$$

$$\beta_0 V_0 \frac{\partial U_L}{\partial r} + \beta_0 \frac{\partial V_0}{\partial r} U_L + V_0 \frac{\partial V_0}{\partial r} R_L = -\frac{1}{r} \frac{\partial P_L}{\partial r} \quad (2)$$

$$\beta_0 V_0 \frac{\partial V_L}{\partial r} + \beta_0 \frac{V_0}{r} V_L = \frac{\beta_L}{r} \frac{1}{r} P_L \quad (3)$$

$$\left[U_L \frac{\partial}{\partial r} + \frac{1}{r^2} \frac{\partial}{\partial r} (r^2 U_L) + \frac{\alpha_L}{r} V_L \right] \left((L+1) \frac{1}{2} \beta_0 V_0^2 + \beta_0 \right) + \left[V_0 \frac{\partial}{\partial r} + \frac{1}{r^2} \frac{\partial}{\partial r} (r^2 V_0) \right] \left((L+1) \frac{1}{2} R_L V_0^2 + (L+1) \beta_0 V_0 U_L + P_L \right) = \frac{2}{\lambda_*} \frac{\partial Q_L}{\partial r} \quad (4)$$

$$\frac{\partial R_L}{\partial r} = \lambda_* \left(R_L q_0 \wedge (\epsilon_0) + \beta_0 Q_L \wedge (\epsilon_0) + \beta_0 q_0 \frac{\partial \lambda}{\partial \epsilon} \Big|_{\epsilon_0} \epsilon_L \right) \quad (5)$$

$$\frac{\partial \epsilon_L}{\partial r} = 2 \lambda_* \left(L(\epsilon_0) R_L + \beta_0 \frac{\partial L}{\partial \epsilon} \Big|_{\epsilon_0} \epsilon_L \right) \quad (6)$$

Boundary conditions

$$T_1(r_p) = 0 \quad U_1(r_p) = 0 \quad V_1(r_p) = 0 \quad Q_1(r_p) = 0 \quad \epsilon_1(r_p) = 0 ?$$

$$P_1(\infty) = 0 \quad R_1(\infty) = 0 \quad Q_1(\infty) = q_0(\infty) \quad \epsilon_1(\infty) = E_0(\infty) \frac{\epsilon_{rel}}{q_{rel}}$$

Put ODE in matrix form $\frac{\partial \vec{Y}}{\partial r} = M \vec{Y}$

$$\text{define } \vec{Y}_1 = \left(P_1, \tau_1, U_1, V_1, Q_1, \epsilon_1 \right)^T$$

$$\text{now use } \alpha_L = -L(L+1) \rightarrow \alpha_1 = -2$$

$$\beta_1 = -1$$

and now abbreviate $\frac{\partial}{\partial r}$ with $()'$

$$(1): \frac{\partial^2}{\partial r^2} U_L + P_L \left[\frac{1}{r^2} \frac{\partial}{\partial r} (r^2 U_L) + \frac{\alpha_L}{r} V_L \right] + V_L \frac{\partial R_L}{\partial r} + \frac{1}{r^2} \frac{\partial}{\partial r} (r^2 V_L) R_L = 0$$

$$\text{with } R_L' = \left(\frac{1}{r} \right)' P_L - \left(\frac{P_L}{r} \right)' \tau_1 + \frac{1}{r} P_L' - \frac{P_L}{r} \tau_1'$$

$$\text{and } (r^2 U_L)' = 2r U_L + r^2 U_L'$$

$$P_L' \left[+ V_0 \left(\frac{1}{r} \right)' + (\vec{V} \cdot \vec{V}_0) \frac{1}{r} \right] + \tau_L' \left[- V_0 \left(\frac{P_L}{r} \right)' - (\vec{V} \cdot \vec{V}_0) \frac{P_L}{r} \right] + U_L' \left[+ P_L' + \beta_0 \frac{P_L}{r} \right] + V_L' \left[- \frac{2 P_L}{r} \right] = P_L' \left[- \frac{V_0}{r} \right] + \tau_L' \left[+ \frac{V_0 P_L}{r} \right] + U_L' \left[+ \beta_0 \right]$$

$$(2): \beta_0 V_0 \frac{\partial U_L}{\partial r} + \beta_0 \frac{\partial V_0}{\partial r} U_L + V_0 \frac{\partial V_0}{\partial r} R_L = -\frac{1}{r} \frac{\partial P_L}{\partial r}$$

$$\Leftrightarrow P_L' \left[V_0 V_0' \frac{1}{r} \right] + \tau_L' \left[- V_0 V_0' \frac{P_L}{r} \right] + U_L' \left[\beta_0 V_0' \right] = P_L' \left[- \frac{1}{r} \right] + U_L' \left[- \beta_0 V_0 \right]$$

$$(3): \beta_0 V_0 \frac{\partial V_L}{\partial r} + \beta_0 \frac{V_0}{r} V_L = \frac{\beta_L}{r} \frac{1}{r} P_L$$

$$\Leftrightarrow P_L' \left[\frac{1}{r} \right] + V_L' \left[\frac{V_0 P_L}{r} \right] = U_L' \left[- \beta_0 V_0 \right] \quad k_L = \left(\frac{1}{r} P_L V_0 + \frac{1}{r} P_L \right)$$

$$(3): \rho_0 v_0 \frac{\partial v_0}{\partial r} + \rho_0 \vec{r} v_0 = \frac{1}{r} \vec{r} p_0$$

$$\Rightarrow p_1 \cdot \left[\frac{1}{r} \right] + v_1 \cdot \left[\frac{v_0}{r} \right] = v_1' \cdot [-\rho_0 v_0] \quad k_0 = \left(\frac{1}{2} \rho_0 v_0^2 + \frac{1}{r} p_0 \right) \quad \vec{v}_0 \cdot \vec{v}_0$$

$$(4): \left[u_1 \frac{\partial}{\partial r} + \frac{1}{r^2} \frac{\partial}{\partial r} (r^2 u_1) + \frac{k_0}{r} v_1 \right] \left[(r-1) \frac{1}{2} \rho_0 v_0^2 + p_0 \right] + \left[v_0 \frac{\partial}{\partial r} + \frac{1}{r^2} \frac{\partial}{\partial r} (r^2 v_0) \right] \left[(r-1) \frac{1}{2} \rho_0 v_0^2 + (r-1) \rho_0 v_0 u_1 + p_1 \right] = \frac{2}{\lambda_*} \frac{\partial Q_1}{\partial r}$$

$$p_1 \cdot \left[(\vec{v}_0 \cdot \vec{v}_0) \left(1 + (r-1) \frac{1}{2} v_0^2 \frac{1}{r} \right) + v_0 (r-1) \frac{1}{2} \left(\frac{v_0^2}{r} \right)' \right] + \tau_1' \cdot \left[-(\vec{v}_0 \cdot \vec{v}_0) (r-1) \frac{1}{2} \frac{\rho_0 v_0^2}{r} - v_0 (r-1) \frac{1}{2} \left(\frac{\rho_0 v_0^2}{r} \right)' \right] \\ + u_1' \cdot \left[k_0' + \frac{2}{r} k_0 + v_0 (r-1) (\rho_0 v_0)' + (\vec{v}_0 \cdot \vec{v}_0) (r-1) \rho_0 v_0 \right] + v_1 \cdot \left[\frac{2 k_0}{r} \right] = p_1' \cdot \left[v_0 - v_0 (r-1) \frac{1}{2} \frac{v_0^2}{r} \right] + \tau_1' \cdot \left[v_0 (r-1) \frac{1}{2} \frac{v_0^2}{r} \right] \\ + u_1' \cdot \left[-k_0 - (r-1) \rho_0 v_0^2 \right] + Q_1' \cdot \left[\frac{2}{\lambda_*} \right] \quad \left| \cdot \frac{1}{r-1} \right.$$

$$\Rightarrow p_1 \cdot \left[(\vec{v}_0 \cdot \vec{v}_0) \left(\frac{1}{r-1} + \frac{1}{2} \frac{v_0^2}{r} \right) + \frac{1}{2} v_0 \left(\frac{v_0^2}{r} \right)' \right] + \tau_1' \cdot \left[-(\vec{v}_0 \cdot \vec{v}_0) \frac{1}{2} \frac{\rho_0 v_0^2}{r} - \frac{1}{2} v_0 \left(\frac{\rho_0 v_0^2}{r} \right)' \right] + u_1' \cdot \left[k_0' + \frac{2}{r} k_0 + v_0 (\rho_0 v_0)' + (\vec{v}_0 \cdot \vec{v}_0) \rho_0 v_0 \right] + v_1 \cdot \left[-\frac{2}{r} k_0 \right] = \\ = p_1' \cdot \left[\frac{v_0}{r-1} - \frac{1}{2} \frac{v_0^3}{r} \right] + \tau_1' \cdot \left[\frac{1}{2} \frac{\rho_0 v_0^3}{r} \right] + u_1' \cdot \left[-k_0 - \rho_0 v_0^2 \right] + Q_1' \cdot \left[\frac{2}{(r-1) \lambda_*} \right]$$

$$(5): \frac{\partial Q_1}{\partial r} = \lambda_* (R_1 q_0 \wedge (\epsilon_0) + \rho_0 Q_1 \wedge (\epsilon_0) + \rho_0 q_1 \frac{\partial \Lambda}{\partial \epsilon} \Big|_{\epsilon_0} \epsilon_1)$$

$$\Rightarrow p_1 \cdot \left[\lambda_* \frac{q_0 \wedge (\epsilon_0)}{r_0} \right] + \tau_1 \cdot \left[\lambda_* \frac{\rho_0 q_0 \wedge (\epsilon_0)}{r_0} \right] + Q_1 \cdot [p_1 \wedge (\epsilon_1)] + \epsilon_1 \cdot \left[\rho_0 q_1 \frac{\partial \Lambda}{\partial \epsilon} \Big|_{\epsilon_1} \right] = Q_1'$$

$$(6): \frac{\partial \epsilon_1}{\partial r} = 2 \lambda_* (L(\epsilon_1) R_1 + \rho_0 \frac{\partial L}{\partial \epsilon} \Big|_{\epsilon_1} \epsilon_1)$$

$$\Rightarrow p_1 \cdot \left[2 \lambda_* \frac{L(\epsilon_1)}{r_0} \right] + \tau_1 \cdot \left[-2 \lambda_* \frac{\rho_0 L(\epsilon_1)}{r_0} \right] + \epsilon_1 \cdot \left[2 \lambda_* \rho_0 \frac{\partial L}{\partial \epsilon} \Big|_{\epsilon_1} \right] = \epsilon_1'$$

In total as the matrix equation $A \vec{\psi} = B \vec{\psi}$
with

$$A = \begin{pmatrix} (1) & p_1' & \tau_1' & u_1' & v_1' & Q_1' & \epsilon_1' \\ (2) & -\frac{v_0}{r} & \frac{v_0 \rho_0}{r_0} & -\rho_0 & 0 & 0 & 0 \\ (3) & -\frac{1}{r} & 0 & -\rho_0 v_0 & 0 & 0 & 0 \\ (4) & 0 & 0 & 0 & -\rho_0 v_0 & 0 & 0 \\ (5) & \left(-\frac{v_0}{r-1} - \frac{1}{2} \frac{v_0^3}{r_0} \right) & \frac{1}{2} \frac{\rho_0 v_0^3}{r_0} & -k_0 - \rho_0 v_0^2 & 0 & \frac{2}{(r-1) \lambda_*} & 0 \\ (6) & 0 & 0 & 0 & 0 & 1 & 0 \\ (7) & 0 & 0 & 0 & 0 & 0 & 1 \end{pmatrix}$$

$$B = \begin{pmatrix} p_1 & \tau_1 & u_1 & v_1 & Q_1 & \epsilon_1 \\ (1) & v_0 \left(\frac{1}{r_0} \right)' + (\vec{v}_0 \cdot \vec{v}_0) \frac{1}{r_0} & -v_0 \left(\frac{\rho_0}{r_0} \right)' - (\vec{v}_0 \cdot \vec{v}_0) \frac{\rho_0}{r_0} & \rho_0' + \frac{2}{r} \rho_0 & -\frac{2}{r} \rho_0 & 0 & 0 \\ (2) & v_0 v_0' \frac{1}{r_0} & -v_0 v_0' \frac{\rho_0}{r_0} & \rho_0 v_0' & 0 & 0 & 0 \\ (3) & \frac{1}{r} & 0 & 0 & \frac{1}{r} v_0 \rho_0 & 0 & 0 \\ (4) & (\vec{v}_0 \cdot \vec{v}_0) \left(\frac{1}{r-1} + \frac{1}{2} \frac{v_0^2}{r} \right) + \frac{1}{2} v_0 \left(\frac{v_0^2}{r_0} \right)' & -(\vec{v}_0 \cdot \vec{v}_0) \frac{1}{2} \frac{\rho_0 v_0^2}{r} - \frac{1}{2} v_0 \left(\frac{\rho_0 v_0^2}{r_0} \right)' & k_0' + \frac{2}{r} k_0 + v_0 (\rho_0 v_0)' + (\vec{v}_0 \cdot \vec{v}_0) \rho_0 v_0 & -\frac{2}{r} k_0 & 0 & 0 \\ (5) & \lambda_* \frac{q_0 \wedge (\epsilon_0)}{r_0} & -\lambda_* \frac{\rho_0 q_0 \wedge (\epsilon_0)}{r_0} & 0 & 0 & \lambda_* \rho_0 \wedge (\epsilon_0) & \lambda_* \rho_0 q_1 \frac{\partial \Lambda}{\partial \epsilon} \Big|_{\epsilon_0} \\ (6) & 2 \lambda_* \frac{L(\epsilon_0)}{r_0} & -2 \lambda_* \frac{\rho_0 L(\epsilon_0)}{r_0} & 0 & 0 & 0 & 2 \lambda_* \rho_0 \frac{\partial L}{\partial \epsilon} \Big|_{\epsilon_0} \end{pmatrix}$$